books/centaur/fgl/bitops-primitives.lisp
@@ -1,0 +1,233 @@
+; GL - A Symbolic Simulation Framework for ACL2
+; Copyright (C) 2018 Centaur Technology
+;
+; Contact:
+;   Centaur Technology Formal Verification Group
+;   7600-C N. Capital of Texas Highway, Suite 300, Austin, TX 78731, USA.
+;   http://www.centtech.com/
+;
+; License: (An MIT/X11-style license)
+;
+;   Permission is hereby granted, free of charge, to any person obtaining a
+;   copy of this software and associated documentation files (the "Software"),
+;   to deal in the Software without restriction, including without limitation
+;   the rights to use, copy, modify, merge, publish, distribute, sublicense,
+;   and/or sell copies of the Software, and to permit persons to whom the
+;   Software is furnished to do so, subject to the following conditions:
+;
+;   The above copyright notice and this permission notice shall be included in
+;   all copies or substantial portions of the Software.
+;
+;   THE SOFTWARE IS PROVIDED "AS IS", WITHOUT WARRANTY OF ANY KIND, EXPRESS OR
+;   IMPLIED, INCLUDING BUT NOT LIMITED TO THE WARRANTIES OF MERCHANTABILITY,
+;   FITNESS FOR A PARTICULAR PURPOSE AND NONINFRINGEMENT. IN NO EVENT SHALL THE
+;   AUTHORS OR COPYRIGHT HOLDERS BE LIABLE FOR ANY CLAIM, DAMAGES OR OTHER
+;   LIABILITY, WHETHER IN AN ACTION OF CONTRACT, TORT OR OTHERWISE, ARISING
+;   FROM, OUT OF OR IN CONNECTION WITH THE SOFTWARE OR THE USE OR OTHER
+;   DEALINGS IN THE SOFTWARE.
+;
+; Original author: Sol Swords <sswords@centtech.com>
+
+(in-package "FGL")
+
+(include-book "primitives")
+(include-book "bitops")
+(local (include-book "primitive-lemmas"))
+(local (include-book "centaur/bitops/ihsext-basics" :dir :system))
+(local (std::add-default-post-define-hook :fix))
+
+
+(def-formula-checks bitops-formula-checks
+  (logapp acl2::logmask$inline acl2::logtail$inline acl2::loghead$inline logbitp))
+
+
+
+(local (defthm fgl-objectlist-eval-when-atom
+         (implies (not (consp x))
+                  (equal (fgl-objectlist-eval x env) nil))
+         :hints(("Goal" :in-theory (enable fgl-objectlist-eval)))))
+
+(local (defthm gobj-bfr-list-eval-of-append
+         (equal (gobj-bfr-list-eval (append x y) env)
+                (append (gobj-bfr-list-eval x env)
+                        (gobj-bfr-list-eval y env)))
+         :hints(("Goal" :in-theory (enable gobj-bfr-list-eval)))))
+
+(local (defthm gobj-bfr-list-eval-of-repeat
+         (equal (gobj-bfr-list-eval (acl2::repeat n x) env)
+                (acl2::repeat n (gobj-bfr-eval x env)))
+         :hints(("Goal" :in-theory (enable gobj-bfr-list-eval acl2::repeat)))))
+
+(local (defthm gobj-bfr-list-eval-of-take
+         (equal (gobj-bfr-list-eval (take n x) env)
+                (take n (gobj-bfr-list-eval x env)))
+         :hints(("Goal" :in-theory (e/d (gobj-bfr-list-eval take acl2::default-cdr)
+                                        (acl2::take-of-zero
+                                         acl2::take-of-too-many))))))
+
+(local (defthm bools->int-of-append
+         (implies (consp y)
+                  (equal (bools->int (append x y))
+                         (logapp (len x) (bools->int x) (bools->int y))))
+         :hints(("Goal" :in-theory (enable bools->int
+                                           bitops::logapp**
+                                           bitops::loghead**
+                                           append len)))))
+
+(local (defthm logcons-bit-identity
+         (implies (bitp b)
+                  (equal (logcons b (- b))
+                         (- b)))
+         :hints(("Goal" :in-theory (enable bitp)))))
+
+(local (defthm logcdr-neg-bit-identity
+         (implies (bitp b)
+                  (equal (logcdr (- b))
+                         (- b)))
+         :hints(("Goal" :in-theory (enable bitp)))))
+
+(define extend-bits ((n natp) x)
+  :guard-hints (("goal" :in-theory (enable default-car)))
+  (b* (((when (zp n)) nil)
+       (first (mbe :logic (car x)
+                   :exec (and (consp x) (car x))))
+       ((when (eql n 1)) (list first))
+       ((when (or (atom x) (atom (cdr x))))
+        (cons first (extend-bits (1- n) x))))
+    (cons first (extend-bits (1- n) (cdr x))))
+  ///
+  (defthm len-of-extend-bits
+    (Equal (len (extend-bits n x)) (nfix n)))
+
+  (defthm consp-of-extend-bits
+    (Equal (consp (extend-bits n x))
+           (posp n)))
+
+  (defthm bools->int-of-extend-bits
+    (equal (bools->int (extend-bits n x))
+           (if (zp n)
+               0
+             (logext n (bools->int x))))
+    :hints(("Goal" :in-theory (enable bools->int bitops::logext**))))
+
+  
+  (local (defthm gobj-bfr-list-eval-under-iff
+           (iff (gobj-bfr-list-eval x env)
+                (consp x))
+           :hints(("Goal" :in-theory (enable gobj-bfr-list-eval)))))
+
+  (defthm gobj-bfr-list-eval-of-extend-bits
+    (equal (gobj-bfr-list-eval (extend-bits n x) env)
+           (extend-bits n (gobj-bfr-list-eval x env)))
+    :hints(("Goal" :in-theory (enable gobj-bfr-list-eval))))
+
+  (defthm member-of-extend-bits
+    (implies (and (not (member v x))
+                  v)
+             (not (member v (extend-bits n x))))))
+
+(local (defthm bools->int-of-repeat
+         (equal (bools->int (acl2::repeat n x))
+                (if (zp n)
+                    0
+                  (- (bool->bit x))))
+         :hints(("Goal" :in-theory (enable bools->int acl2::repeat)))))
+
+(local (defthm logapp-bools->int-of-extend-bits
+         (equal (logapp n (bools->int (extend-bits n x)) y)
+                (logapp n (bools->int x) y))
+         :hints(("Goal" :in-theory (enable bools->int
+                                           bitops::logapp**
+                                           bitops::logext**
+                                           take)))))
+
+(local (defthm fgl-object-eval-when-atom-gobj-syntactic-integer->bits
+         (b* (((mv ok fix) (gobj-syntactic-integer-fix x)))
+           (implies (and ok
+                         (not (gobj-syntactic-integer->bits fix)))
+                    (acl2::int-equiv (fgl-object-eval x env) 0)))
+         :hints (("goal" :use ((:instance fgl-object-eval-of-gobj-syntactic-integer-fix))
+                  :in-theory (disable fgl-object-eval-of-gobj-syntactic-integer-fix)))))
+
+(local (in-theory (enable bitops::logapp** bitops::loghead** bitops::logtail**)))
+
+(set-ignore-ok t)
+
+(def-gl-primitive logapp (width lsbs msbs)
+  (b* (((unless (gl-object-case width :g-concrete))
+        (mv nil nil interp-st))
+       ((mv ok lsbs) (gobj-syntactic-integer-fix lsbs))
+       ((unless ok) (mv nil nil interp-st))
+       ((mv ok msbs) (gobj-syntactic-integer-fix msbs))
+       ((unless ok) (mv nil nil interp-st))
+       (lsb-bits (gobj-syntactic-integer->bits lsbs))
+       (msb-bits (gobj-syntactic-integer->bits msbs)))
+    (mv t (mk-g-integer (append (extend-bits (nfix (g-concrete->val width))
+                                             lsb-bits)
+                                (if (atom msb-bits) '(nil) msb-bits)))
+        interp-st))
+  :formula-check bitops-formula-checks)
+
+(define tail-bits ((n natp) x)
+  (b* (((when (zp n)) x)
+       ((when (mbe :logic (atom (cdr x))
+                   :exec (or (atom x) (atom (cdr x)))))
+        x))
+    (tail-bits (1- n) (cdr x)))
+  ///
+  (local (defthm logtail-neg-bit
+           (implies (bitp b)
+                    (equal (logtail n (- b))
+                           (- b)))
+           :hints(("Goal" :in-theory (enable* bitops::logtail**
+                                              bitops::ihsext-inductions)))))
+
+  (defthm bools->int-of-tail-bits
+    (equal (bools->int (tail-bits n x))
+           (logtail n (bools->int x)))
+    :hints(("Goal" :in-theory (enable bools->int bitops::logtail**))))
+
+  
+
+  (defthm gobj-bfr-list-eval-of-tail-bits
+    (equal (gobj-bfr-list-eval (tail-bits n x) env)
+           (tail-bits n (gobj-bfr-list-eval x env)))
+    :hints(("Goal" :in-theory (enable gobj-bfr-list-eval))))
+
+  (defthm member-of-tail-bits
+    (implies (not (member v x))
+             (not (member v (tail-bits n x)))))
+
+  (defthm true-listp-of-tail-bits
+    (iff (true-listp (tail-bits n x))
+         (true-listp x))))
+
+(def-gl-primitive acl2::logtail$inline (n x)
+  (b* (((unless (gl-object-case n :g-concrete))
+        (mv nil nil interp-st))
+       ((mv ok x) (gobj-syntactic-integer-fix x))
+       ((unless ok) (mv nil nil interp-st))
+       (x-bits (gobj-syntactic-integer->bits x)))
+    (mv t (mk-g-integer (tail-bits (nfix (g-concrete->val n)) x-bits))
+        interp-st))
+  :formula-check bitops-formula-checks)
+
+
+
+(local (install-gl-primitives logapp))
+(remove-gl-rewrite logapp-const-width)
+(remove-gl-rewrite logtail-const-shift)
+
+(def-gl-rewrite logapp-const-width-allow-primitive
+  (implies (syntaxp (and (integerp n)
+                         ;; Allow this only when x is a g-var or g-apply, so
+                         ;; that the primitive would fail but this can
+                         ;; potentially generate bits for x.
+                         (gl-object-case x '(:g-var :g-apply))))
+           (equal (logapp n x y)
+                  (cond ((zp n) (int y))
+                        (t (intcons (and (intcar x) t)
+                                    (logapp (1- n) (intcdr x) y))))))
+  :hints(("Goal" :in-theory (enable intcons intcar intcdr int-endp
+                                    bitops::logapp**))))
+
